theories/ccompiler/equiv.v
@@ -1,10 +1,14 @@
-From Wasm Require Import datatypes.
+Require Import Coq.Lists.List.
+Import ListNotations.
+From Wasm Require Import datatypes opsem.
 From Wasm Require Import ccompiler.compile ccompiler.num_conv.
 Require Import compcert.lib.Integers.
 Require Import compcert.cfrontend.Clight.
 Require Import compcert.common.AST.
 Require Import compcert.common.Memory.
 Require Import compcert.common.Values.
+Require Import compcert.common.Events.
+Require Import compcert.lib.Maps.
 
 Definition val_equiv (v : value) : val :=
   match v with
@@ -14,10 +18,23 @@ Definition val_equiv (v : value) : val :=
   | VAL_float64 x => Vfloat x
   end.
 
-Lemma lit_equiv :
-  forall (ge : genv) (e : env) (te : temp_env) (m : mem),
-  forall (c : value),
-  eval_expr ge e te m (compile_value c) (val_equiv c).
+Lemma value_equiv :
+  forall (ge : genv) (e : env) (le : temp_env) (m : mem),
+  forall c : value,
+  eval_expr ge e le m (compile_value c) (val_equiv c).
 Proof.
   intros. unfold compile_value. destruct c; eauto using eval_expr.
 Qed.
+
+  (* TODO: reflexive transitive closure of Clight.step *)
+Lemma unop_equiv :
+  forall (ge : genv) (function_entry : function -> list val -> mem -> env -> temp_env -> mem -> Prop) (f : function) (k : cont) (e : env) (m : mem)
+         (vt : value_type) (u : unop) (r : ident) (x : ident) (v v' : value)
+         (le le' : temp_env) (s : statement),
+  reduce_simple [AI_basic (BI_const v); AI_basic (BI_unop vt u)]
+                [AI_basic (BI_const v')] ->
+  compile_unop vt u r x = Some s ->
+  step ge function_entry (State f s k e le m) E0 (State f Sskip k e le' m) ->
+  PTree.get x le = Some (val_equiv v) ->
+  PTree.get r le' = Some (val_equiv v').
+Proof.
